Deque/deque.v
@@ -14,6 +14,11 @@ From Deque Require Import buffer.
 Inductive preferred_child : Type :=
   | Preferred : bool -> bool -> preferred_child.
 
+Notation preferred_left := (Preferred true false).
+Notation preferred_right := (Preferred false true).
+
+Derive NoConfusion for preferred_child.
+
 Inductive kind : Type := Only | Left | Right.
 
 (* Here, [green_hue], [yellow_hue], [orange_hue] and [red_hue] will be utilized 
@@ -55,9 +60,9 @@ Definition prefix' := buffer.t.
 Definition suffix' := buffer.t.
 
 Inductive small_triple_size : nat -> nat -> kind -> Type :=
-  | POnly {q : nat} : small_triple_size (S q) 0 Only
-  | PLeft {q : nat} : small_triple_size (5 + q) 2 Left
-  | PRight {q : nat} : small_triple_size 2 (5 + q) Right.
+  | SOnly {q : nat} : small_triple_size (S q) 0 Only
+  | SLeft {q : nat} : small_triple_size (5 + q) 2 Left
+  | SRight {q : nat} : small_triple_size 2 (5 + q) Right.
 
 Inductive big_triple_size : nat -> nat -> nat -> kind -> Type :=
   | BOnly {p qp qs : nat} : big_triple_size p (p + qp) (p + qs) Only
@@ -85,25 +90,25 @@ with triple (A : Type) : nat -> nat -> bool -> kind -> kind -> color -> Type :=
       triple A lvl 0 false K K green
   | Green {lvl qp qs : nat} {K : kind} {G R} :
       prefix' (stored_triple A lvl) qp ->
-      cdeque A (S lvl) (Mix G NoYellow NoOrange R) ->
+      non_empty_cdeque A (S lvl) (Mix G NoYellow NoOrange R) ->
       suffix' (stored_triple A lvl) qs ->
       big_triple_size 8 qp qs K ->
       triple A lvl 0 false K K green
   | Yellow {lvl len qp qs : nat} {K1 K2 : kind} :
       prefix' (stored_triple A lvl) qp ->
-      packet A (S lvl) len (Preferred true false) K2 ->
+      packet A (S lvl) len preferred_left K2 ->
       suffix' (stored_triple A lvl) qs ->
       big_triple_size 7 qp qs K1 ->
       triple A lvl (S len) false K1 K2 yellow
   | Orange {lvl len qp qs : nat} {K1 K2 : kind} :
       prefix' (stored_triple A lvl) qp ->
-      packet A (S lvl) len (Preferred false true) K2 ->
+      packet A (S lvl) len preferred_right K2 ->
       suffix' (stored_triple A lvl) qs ->
       big_triple_size 6 qp qs K1 ->
       triple A lvl (S len) false K1 K2 orange
   | Red {lvl qp qs : nat} {K : kind} :
       prefix' (stored_triple A lvl) qp ->
-      cdeque A (S lvl) green ->
+      non_empty_cdeque A (S lvl) green ->
       suffix' (stored_triple A lvl) qs ->
       big_triple_size 5 qp qs K ->
       triple A lvl 0 false K K red
@@ -115,11 +120,11 @@ with packet (A : Type) : nat -> nat -> preferred_child -> kind -> Type :=
   | Left_child {lvl len : nat} {is_hole : bool} {K : kind} {Y O C} :
       triple A lvl len is_hole Left K (Mix NoGreen Y O NoRed) ->
       path A lvl Right C ->
-      packet A lvl len (Preferred true false) K
+      packet A lvl len preferred_left K
   | Right_child {lvl len : nat} {is_hole : bool} {K : kind} {Y O} :
       path A lvl Left green ->
       triple A lvl len is_hole Right K (Mix NoGreen Y O NoRed) ->
-      packet A lvl len (Preferred false true) K
+      packet A lvl len preferred_right K
 
 with path (A : Type) : nat -> kind -> color -> Type := 
   | Children {lvl len nlvl : nat} {is_hole : bool} {K1 K2 : kind} {G Y O R} :
@@ -128,19 +133,24 @@ with path (A : Type) : nat -> kind -> color -> Type :=
       nlvl = len + lvl ->
       path A lvl K1 (Mix G NoYellow NoOrange R)
 
-with cdeque (A : Type) : nat -> color -> Type :=
-  | Empty {lvl : nat} : cdeque A lvl green 
+with non_empty_cdeque (A : Type) : nat -> color -> Type :=
   | Only_path {lvl : nat} {G R} :
       path A lvl Only (Mix G NoYellow NoOrange R) ->
-      cdeque A lvl (Mix G NoYellow NoOrange R)
+      non_empty_cdeque A lvl (Mix G NoYellow NoOrange R)
   | Pair_green {lvl : nat} :
       path A lvl Left green ->
       path A lvl Right green ->
-      cdeque A lvl green
+      non_empty_cdeque A lvl green
   | Pair_red {lvl : nat} {Cl Cr : color} :
       path A lvl Left Cl ->
       path A lvl Right Cr ->
-      cdeque A lvl red.
+      non_empty_cdeque A lvl red
+
+with cdeque (A : Type) : nat -> color -> Type :=
+  | Empty {lvl : nat} : cdeque A lvl green
+  | NonEmpty {lvl G R} : 
+      non_empty_cdeque A lvl (Mix G NoYellow NoOrange R) ->
+      cdeque A lvl (Mix G NoYellow NoOrange R).
 
 Arguments ST_ground {A}.
 Arguments ST_small {A lvl q}.
@@ -159,10 +169,12 @@ Arguments Right_child {A lvl len is_hole K Y O}.
 
 Arguments Children {A lvl len nlvl is_hole K1 K2 G Y O R}.
 
-Arguments Empty {A lvl}.
 Arguments Only_path {A lvl G R}.
 Arguments Pair_green {A lvl}.
 Arguments Pair_red {A lvl Cl Cr}.
+
+Arguments Empty {A lvl}.
+Arguments NonEmpty {A lvl G R}.
 
 Definition prefix (A : Type) (lvl : nat) := prefix' (stored_triple A lvl).
 Definition suffix (A : Type) (lvl : nat) := suffix' (stored_triple A lvl).
@@ -174,9 +186,70 @@ Definition left_triple (A : Type) (lvl len : nat) (is_hole : bool) :=
 Definition right_triple (A : Type) (lvl len : nat) (is_hole : bool) := 
   triple A lvl len is_hole Right.
 
+Inductive pref_left (A : Type) (lvl : nat) : Type :=
+  | Pref_left {len nlvl K G R} : 
+      packet A lvl len preferred_left K ->
+      triple A nlvl 0 false K K (Mix G NoYellow NoOrange R) ->
+      nlvl = len + lvl ->
+      pref_left A lvl.
+Arguments Pref_left {A lvl len nlvl K G R}.
+
+Inductive pref_right (A : Type) (lvl : nat) : Type :=
+  | Pref_right {len nlvl K G R} :
+      packet A lvl len preferred_right K ->
+      triple A nlvl 0 false K K (Mix G NoYellow NoOrange R) ->
+      nlvl = len + lvl ->
+      pref_right A lvl.
+Arguments Pref_right {A lvl len nlvl K G R}.
+
+Definition buffer_12 (A : Type) (lvl : nat) : Type := stored_triple A lvl * vector (stored_triple A lvl) 1.
+
+Inductive path_attempt (A : Type) (lvl : nat) : kind -> color -> Type :=
+  | ZeroSix {K : kind} {C : color} : 
+      vector (stored_triple A lvl) 6 -> path_attempt A lvl K C
+  | Ok {K : kind} {C : color} : 
+      path A lvl K C -> path_attempt A lvl K C
+  | Any {K : kind} {C : color} :
+      path A lvl K C -> path_attempt A lvl K red.
+Arguments ZeroSix {A lvl K C}.
+Arguments Ok {A lvl K C}.
+Arguments Any {A lvl K C}.
+
+Inductive path_uncolored (A : Type) (lvl : nat) (K : kind) : Type :=
+  | Six : stored_triple A lvl -> stored_triple A lvl -> stored_triple A lvl ->
+          stored_triple A lvl -> stored_triple A lvl -> stored_triple A lvl ->
+          path_uncolored A lvl K
+  | AnyColor {C : color} : path A lvl K C -> path_uncolored A lvl K.
+Arguments Six {A lvl K}.
+Arguments AnyColor {A lvl K C}.
+
 Inductive sdeque (A : Type) (lvl : nat) : Type :=
   Sd : forall (C : color), cdeque A lvl C -> sdeque A lvl.
 Arguments Sd {A lvl C}.
+
+Inductive unstored (A : Type) (lvl : nat) : Type :=
+  | Unstored {q : nat} : 
+      prefix A lvl (3 + q) -> sdeque A (S lvl) -> unstored A lvl.
+Arguments Unstored {A lvl q}.
+
+Inductive sandwich (A : Type) (lvl : nat) : Type :=
+  | Alone : stored_triple A lvl -> sandwich A lvl
+  | Sandwich : 
+      stored_triple A lvl -> sdeque A lvl -> stored_triple A lvl ->
+      sandwich A lvl.
+Arguments Alone {A lvl}.
+Arguments Sandwich {A lvl}.
+
+Inductive unstored_sandwich (A : Type) (lvl : nat) : Type :=
+  | Unstored_alone {q : nat} :
+      prefix A lvl (3 + q) -> unstored_sandwich A lvl
+  | Unstored_sandwich {qp qs : nat} :
+      prefix A lvl (3 + qp) -> 
+      sdeque A (S lvl) ->
+      suffix A lvl (3 + qs) ->
+      unstored_sandwich A lvl.
+Arguments Unstored_alone {A lvl q}.
+Arguments Unstored_sandwich {A lvl qp qs}.
 
 Inductive deque (A : Type) : Type :=
   T : cdeque A 0 green -> deque A.
@@ -189,11 +262,8 @@ Set Equations Transparent.
 Parameter stored_triple_seq : 
   forall {A lvl}, stored_triple A lvl -> list A.
 
-Equations prefix_seq {A lvl q} : prefix A lvl q -> list A :=
-prefix_seq p := concat (map stored_triple_seq (buffer.seq p)).
-
-Equations suffix_seq {A lvl q} : suffix A lvl q -> list A :=
-suffix_seq s := concat (map stored_triple_seq (buffer.seq s)).
+Equations buffer_seq {A lvl q} : buffer.t (stored_triple A lvl) q -> list A :=
+buffer_seq p := concat (map stored_triple_seq (buffer.seq p)).
 
 Parameter triple_front_seq :
   forall {A lvl len is_hole K1 K2 C}, 
@@ -204,18 +274,21 @@ Parameter triple_rear_seq :
   triple A lvl len is_hole K1 K2 C -> list A.
 
 Equations triple_seq {A lvl len is_hole K1 K2 C} : 
-  triple A lvl len is_hole K1 K2 C -> list A :=
+  triple A lvl len is_hole K1 K2 C -> list A := 
 triple_seq t := triple_front_seq t ++ triple_rear_seq t.
 
 Equations path_seq {A lvl K C} : path A lvl K C -> list A :=
 path_seq (Children nchild achild _) := 
   triple_front_seq nchild ++ triple_seq achild ++ triple_rear_seq nchild.
 
+Equations ne_cdeque_seq {A lvl C} : non_empty_cdeque A lvl C -> list A :=
+ne_cdeque_seq (Only_path p) := path_seq p;
+ne_cdeque_seq (Pair_green p1 p2) := path_seq p1 ++ path_seq p2;
+ne_cdeque_seq (Pair_red p1 p2) := path_seq p1 ++ path_seq p2.
+
 Equations cdeque_seq {A lvl C} : cdeque A lvl C -> list A :=
 cdeque_seq Empty := [];
-cdeque_seq (Only_path p) := path_seq p;
-cdeque_seq (Pair_green p1 p2) := path_seq p1 ++ path_seq p2;
-cdeque_seq (Pair_red p1 p2) := path_seq p1 ++ path_seq p2.
+cdeque_seq (NonEmpty cd) := ne_cdeque_seq cd.
 
 Equations packet_front_seq {A lvl len pc K} : packet A lvl len pc K -> list A :=
 packet_front_seq (Only_child child) := triple_front_seq child;
@@ -227,21 +300,63 @@ packet_rear_seq (Only_child child) := triple_rear_seq child;
 packet_rear_seq (Left_child child path) := triple_rear_seq child ++ path_seq path;
 packet_rear_seq (Right_child _ child) := triple_rear_seq child.
 
+Equations pref_left_seq {A lvl} : pref_left A lvl -> list A :=
+pref_left_seq (Pref_left pkt t eq_refl) := packet_front_seq pkt ++ triple_seq t ++ packet_rear_seq pkt.
+
+Equations pref_right_seq {A lvl} : pref_right A lvl -> list A :=
+pref_right_seq (Pref_right pkt t eq_refl) := packet_front_seq pkt ++ triple_seq t ++ packet_rear_seq pkt.
+
+Equations buffer_12_seq {A lvl} : buffer_12 A lvl -> list A :=
+buffer_12_seq (x, v) := stored_triple_seq x ++ concat (map stored_triple_seq (vector_seq v)).
+
+Equations path_attempt_seq {A lvl K C} : path_attempt A lvl K C -> list A :=
+path_attempt_seq (ZeroSix v) := concat (map stored_triple_seq (vector_seq v));
+path_attempt_seq (Ok p) := path_seq p;
+path_attempt_seq (Any p) := path_seq p.
+
+Equations path_uncolored_seq {A lvl K} : path_uncolored A lvl K -> list A :=
+path_uncolored_seq (Six x1 x2 x3 x4 x5 x6) := 
+  stored_triple_seq x1 ++ stored_triple_seq x2 ++ stored_triple_seq x3 ++
+  stored_triple_seq x4 ++ stored_triple_seq x5 ++ stored_triple_seq x6;
+path_uncolored_seq (AnyColor p) := path_seq p. 
+
+Equations sdeque_seq {A lvl} : sdeque A lvl -> list A :=
+sdeque_seq (Sd cd) := cdeque_seq cd.
+
+Equations unstored_front_seq {A lvl} : unstored A lvl -> list A :=
+unstored_front_seq (Unstored p _) := buffer_seq p.
+
+Equations unstored_rear_seq {A lvl} : unstored A lvl -> list A :=
+unstored_rear_seq (Unstored _ sd) := sdeque_seq sd.
+
+Equations sandwich_seq {A lvl} : sandwich A lvl -> list A :=
+sandwich_seq (Alone x) := stored_triple_seq x;
+sandwich_seq (Sandwich xl sd xr) :=
+  stored_triple_seq xl ++ sdeque_seq sd ++ stored_triple_seq xr.
+
+Equations unstored_sandwich_seq {A lvl} : unstored_sandwich A lvl -> list A :=
+unstored_sandwich_seq (Unstored_alone p) := buffer_seq p;
+unstored_sandwich_seq (Unstored_sandwich p sd s) := 
+  buffer_seq p ++ sdeque_seq sd ++ buffer_seq s.
+
 Equations deque_seq {A} : deque A -> list A :=
 deque_seq (T cd) := cdeque_seq cd.
 
 Unset Equations Transparent.
 
+Axiom stored_triple_ground : forall [A], forall (x : A),
+  stored_triple_seq (ST_ground x) = [x].
+
 Axiom stored_triple_small : forall [A lvl q], forall 
   (p : prefix A lvl (3 + q)),
-  stored_triple_seq (ST_small p) = prefix_seq p.
+  stored_triple_seq (ST_small p) = buffer_seq p.
   
 Axiom stored_triple_triple : forall [A lvl qp qs C], forall 
   (p : prefix A lvl (3 + qp)) 
   (cd : cdeque A (S lvl) C) 
   (s : suffix A lvl (3 + qs)),
   stored_triple_seq (ST_triple p cd s) =
-    prefix_seq p ++ cdeque_seq cd ++ suffix_seq s.
+    buffer_seq p ++ cdeque_seq cd ++ buffer_seq s.
 
 Axiom triple_front_hole : forall (A : Type) (lvl : nat) (K : kind), 
   triple_front_seq (A := A) (lvl := lvl) (K1 := K) Hole = [].
@@ -253,73 +368,73 @@ Axiom triple_front_small : forall [A lvl qp qs K], forall
   (p : prefix A lvl qp)
   (s : suffix A lvl qs)
   (ss : small_triple_size qp qs K),
-  triple_front_seq (Small p s ss) = prefix_seq p.
+  triple_front_seq (Small p s ss) = buffer_seq p.
 
-Axiom triple_rear_small : forall [A lvl qp qs K], forall 
+Axiom triple_rear_small : forall [A lvl qp qs K], forall
   (p : prefix A lvl qp)
   (s : suffix A lvl qs)
   (ss : small_triple_size qp qs K),
-  triple_rear_seq (Small p s ss) = suffix_seq s.
+  triple_rear_seq (Small p s ss) = buffer_seq s.
 
 Axiom triple_front_green : forall [A lvl qp qs K G R], forall
   (p : prefix A lvl qp)
-  (cd : cdeque A (S lvl) (Mix G NoYellow NoOrange R))
+  (cd : non_empty_cdeque A (S lvl) (Mix G NoYellow NoOrange R))
   (s : suffix A lvl qs)
   (bs : big_triple_size 8 qp qs K),
-  triple_front_seq (Green p cd s bs) = prefix_seq p ++ cdeque_seq cd.
+  triple_front_seq (Green p cd s bs) = buffer_seq p ++ ne_cdeque_seq cd.
 
 Axiom triple_rear_green : forall [A lvl qp qs K G R], forall
   (p : prefix A lvl qp)
-  (cd : cdeque A (S lvl) (Mix G NoYellow NoOrange R))
+  (cd : non_empty_cdeque A (S lvl) (Mix G NoYellow NoOrange R))
   (s : suffix A lvl qs)
   (bs : big_triple_size 8 qp qs K),
-  triple_rear_seq (Green p cd s bs) = suffix_seq s.
+  triple_rear_seq (Green p cd s bs) = buffer_seq s.
 
 Axiom triple_front_yellow : forall [A lvl len qp qs K1 K2], forall
   (p : prefix A lvl qp)
-  (pkt : packet A (S lvl) len (Preferred true false) K2)
+  (pkt : packet A (S lvl) len preferred_left K2)
   (s : suffix A lvl qs)
   (bs : big_triple_size 7 qp qs K1),
   triple_front_seq (Yellow p pkt s bs) =
-    prefix_seq p ++ packet_front_seq pkt.
+    buffer_seq p ++ packet_front_seq pkt.
 
 Axiom triple_rear_yellow : forall [A lvl len qp qs K1 K2], forall
   (p : prefix A lvl qp)
-  (pkt : packet A (S lvl) len (Preferred true false) K2)
+  (pkt : packet A (S lvl) len preferred_left K2)
   (s : suffix A lvl qs)
   (bs : big_triple_size 7 qp qs K1),
   triple_rear_seq (Yellow p pkt s bs) =
-    packet_rear_seq pkt ++ suffix_seq s.
+    packet_rear_seq pkt ++ buffer_seq s.
 
 Axiom triple_front_orange : forall [A lvl len qp qs K1 K2], forall
   (p : prefix A lvl qp)
-  (pkt : packet A (S lvl) len (Preferred false true) K2)
+  (pkt : packet A (S lvl) len preferred_right K2)
   (s : suffix A lvl qs)
   (bs : big_triple_size 6 qp qs K1),
   triple_front_seq (Orange p pkt s bs) =
-    prefix_seq p ++ packet_front_seq pkt.
+    buffer_seq p ++ packet_front_seq pkt.
 
 Axiom triple_rear_orange : forall [A lvl len qp qs K1 K2], forall
   (p : prefix A lvl qp)
-  (pkt : packet A (S lvl) len (Preferred false true) K2)
+  (pkt : packet A (S lvl) len preferred_right K2)
   (s : suffix A lvl qs)
   (bs : big_triple_size 6 qp qs K1),
   triple_rear_seq (Orange p pkt s bs) =
-    packet_rear_seq pkt ++ suffix_seq s.
+    packet_rear_seq pkt ++ buffer_seq s.
 
 Axiom triple_front_red : forall [A lvl qp qs K], forall
   (p : prefix A lvl qp)
-  (cd : cdeque A (S lvl) green)
+  (cd : non_empty_cdeque A (S lvl) green)
   (s : suffix A lvl qs)
   (bs : big_triple_size 5 qp qs K),
-  triple_front_seq (Red p cd s bs) = prefix_seq p ++ cdeque_seq cd.
+  triple_front_seq (Red p cd s bs) = buffer_seq p ++ ne_cdeque_seq cd.
 
 Axiom triple_rear_red : forall [A lvl qp qs K], forall
   (p : prefix A lvl qp)
-  (cd : cdeque A (S lvl) green)
+  (cd : non_empty_cdeque A (S lvl) green)
   (s : suffix A lvl qs)
   (bs : big_triple_size 5 qp qs K),
-  triple_rear_seq (Red p cd s bs) = suffix_seq s.
+  triple_rear_seq (Red p cd s bs) = buffer_seq s.
 
 (* The list application is made opaque. *)
 
@@ -336,6 +451,7 @@ Opaque singleton.
 #[export] Hint Rewrite map_app : rlist.
 #[export] Hint Rewrite concat_app : rlist.
 
+#[export] Hint Rewrite stored_triple_ground : rlist.
 #[export] Hint Rewrite stored_triple_small : rlist.
 #[export] Hint Rewrite stored_triple_triple : rlist.
 #[export] Hint Rewrite triple_front_hole : rlist.
@@ -353,16 +469,16 @@ Opaque singleton.
 
 (* Lemmas *)
 
-Lemma empty_prefix [A lvl] (p : prefix A lvl 0) : prefix_seq p = [].
+Lemma empty_prefix [A lvl] (p : prefix A lvl 0) : buffer_seq p = [].
 Proof.
-  unfold prefix_seq; unfold prefix, prefix' in p.
+  unfold buffer_seq; unfold prefix, prefix' in p.
   pose buffer.empty_buffer as H; rewrite H.
   reflexivity.
 Qed.
 
-Lemma empty_suffix [A lvl] (s : suffix A lvl 0) : suffix_seq s = [].
+Lemma empty_suffix [A lvl] (s : suffix A lvl 0) : buffer_seq s = [].
 Proof. 
-  unfold suffix_seq; unfold suffix, suffix' in s. 
+  unfold buffer_seq; unfold suffix, suffix' in s. 
   pose buffer.empty_buffer as H; rewrite H.
   reflexivity.
 Qed.
@@ -370,7 +486,12 @@ Qed.
 #[export] Hint Rewrite empty_buffer : rlist.
 
 #[local] Obligation Tactic :=
-  try first [ done | cbn; hauto db:rlist ].
+  try first [ done | 
+    cbn beta iota delta zeta; intros; 
+    try simp triple_seq in *;
+    autorewrite with rlist;
+    try simp buffer_seq in *;
+    hauto db:rlist ].
 
 Notation "? x" := (@exist _ _ x _) (at level 100).
 
@@ -381,93 +502,1050 @@ empty := ? T Empty.
 
 (* Functions *)
 
+Equations push_seq_equality {A lvl len K1 K2 C} 
+  (x : stored_triple A lvl)
+  (t1 t2 : triple A lvl len false K1 K2 C) : Prop :=
+push_seq_equality (C := Mix _ NoYellow NoOrange _) x t1 t2 := 
+  triple_seq t2 = stored_triple_seq x ++ triple_seq t1;
+push_seq_equality (C := Mix NoGreen _ _ NoRed) x t1 t2 :=
+  triple_front_seq t2 = stored_triple_seq x ++ triple_front_seq t1 
+  /\ triple_rear_seq t2 = triple_rear_seq t1.
+Transparent push_seq_equality.
+
+Equations inject_seq_equality {A lvl len K1 K2 C} 
+  (t1 : triple A lvl len false K1 K2 C)
+  (x : stored_triple A lvl)
+  (t2 : triple A lvl len false K1 K2 C) : Prop :=
+inject_seq_equality (C := Mix _ NoYellow NoOrange _) t1 x t2 := 
+  triple_seq t2 = triple_seq t1 ++ stored_triple_seq x;
+inject_seq_equality (C := Mix NoGreen _ _ NoRed) t1 x t2 :=
+  triple_front_seq t2 = triple_front_seq t1 /\
+  triple_rear_seq t2 = triple_rear_seq t1 ++ stored_triple_seq x.
+Transparent inject_seq_equality.
+
 Equations push_only_triple {A lvl len K C}
   (x : stored_triple A lvl) 
   (t : only_triple A lvl len false K C) :
-  { t' : only_triple A lvl len false K C | 
-    triple_seq t' = stored_triple_seq x ++ triple_seq t } :=
-push_only_triple x (Small p s POnly) with buffer.push x p => {
-  | ? p' := ? Small p' s POnly };
+  { t' : only_triple A lvl len false K C | push_seq_equality x t t' } :=
+push_only_triple x (Small p s SOnly) with buffer.push x p => {
+  | ? p' := ? Small p' s SOnly };
 push_only_triple x (Green p cd s BOnly) with buffer.push x p => {
   | ? p' := ? Green p' cd s BOnly };
-push_only_triple x (Yellow p cd s BOnly) with buffer.push x p => {
-  | ? p' := ? Yellow p' cd s BOnly };
-push_only_triple x (Orange p cd s BOnly) with buffer.push x p => {
-  | ? p' := ? Orange p' cd s BOnly };
+push_only_triple x (Yellow p pkt s BOnly) with buffer.push x p => {
+  | ? p' := ? Yellow p' pkt s BOnly };
+push_only_triple x (Orange p pkt s BOnly) with buffer.push x p => {
+  | ? p' := ? Orange p' pkt s BOnly };
 push_only_triple x (Red p cd s BOnly) with buffer.push x p => {
   | ? p' := ? Red p' cd s BOnly }.
-Next Obligation.
-  cbn; intros * Hbuf *; simp triple_seq.
-  autorewrite with rlist; simp prefix_seq; hauto db:rlist.
-Qed.
-Next Obligation.
-  cbn; intros * Hbuf *; simp triple_seq.
-  autorewrite with rlist; simp prefix_seq; hauto db:rlist.
-Qed.
-Next Obligation.
-  cbn; intros * Hbuf *; simp triple_seq.
-  autorewrite with rlist; simp prefix_seq; hauto db:rlist.
-Qed.
-Next Obligation.
-  cbn; intros * Hbuf *; simp triple_seq.
-  autorewrite with rlist; simp prefix_seq; hauto db:rlist.
-Qed.
-Next Obligation.
-  cbn; intros * Hbuf *; simp triple_seq.
-  autorewrite with rlist; simp prefix_seq; hauto db:rlist.
-Qed.
 
 Equations inject_only_triple {A lvl len K C}
   (t : only_triple A lvl len false K C)
   (x : stored_triple A lvl) :
-  { t' : only_triple A lvl len false K C | 
-    triple_seq t' = triple_seq t ++ stored_triple_seq x } :=
-inject_only_triple (Small p s POnly) x with buffer.inject p x => {
-  | ? p' := ? Small p' s POnly };
+  { t' : only_triple A lvl len false K C | inject_seq_equality t x t' } :=
+inject_only_triple (Small p s SOnly) x with buffer.inject p x => {
+  | ? p' := ? Small p' s SOnly };
 inject_only_triple (Green p cd s BOnly) x with buffer.inject s x => {
   | ? s' := ? Green p cd s' BOnly };
-inject_only_triple (Yellow p cd s BOnly) x with buffer.inject s x => {
-  | ? s' := ? Yellow p cd s' BOnly };
-inject_only_triple (Orange p cd s BOnly) x with buffer.inject s x => {
-  | ? s' := ? Orange p cd s' BOnly };
+inject_only_triple (Yellow p pkt s BOnly) x with buffer.inject s x => {
+  | ? s' := ? Yellow p pkt s' BOnly };
+inject_only_triple (Orange p pkt s BOnly) x with buffer.inject s x => {
+  | ? s' := ? Orange p pkt s' BOnly };
 inject_only_triple (Red p cd s BOnly) x with buffer.inject s x => {
   | ? s' := ? Red p cd s' BOnly }.
-Next Obligation.
-  cbn; intros * Hbuf *; simp triple_seq.
-  autorewrite with rlist; simp prefix_seq; hauto db:rlist.
-Qed.
-Next Obligation.
-  cbn; intros * Hbuf *; simp triple_seq.
-  autorewrite with rlist; simp prefix_seq; hauto db:rlist.
-Qed.
-Next Obligation.
-  cbn; intros * Hbuf *; simp triple_seq.
-  autorewrite with rlist; simp prefix_seq; hauto db:rlist.
-Qed.
-Next Obligation.
-  cbn; intros * Hbuf *; simp triple_seq.
-  autorewrite with rlist; simp prefix_seq; hauto db:rlist.
-Qed.
-Next Obligation.
-  cbn; intros * Hbuf *; simp triple_seq.
-  autorewrite with rlist; simp prefix_seq; hauto db:rlist.
-Qed.
 
 Equations push_only_path {A lvl C} 
   (x : stored_triple A lvl) 
   (p : path A lvl Only C) :
   { p' : path A lvl Only C | path_seq p' = stored_triple_seq x ++ path_seq p } :=
-push_only_path x (Children Hole adoptive eq_refl) with push_only_triple x adoptive => {
-  | ? adoptive' := ? Children Hole adoptive' eq_refl };
+push_only_path x (Children Hole natural eq_refl) with push_only_triple x natural => {
+  | ? natural' := ? Children Hole natural' eq_refl };
 push_only_path x (Children natural adoptive eq_refl) with push_only_triple x natural => {
   | ? natural' := ? Children natural' adoptive eq_refl }.
+
+Equations inject_only_path {A lvl C}
+  (p : path A lvl Only C)
+  (x : stored_triple A lvl) :
+  { p' : path A lvl Only C | path_seq p' = path_seq p ++ stored_triple_seq x } :=
+inject_only_path (Children Hole adoptive eq_refl) x with inject_only_triple adoptive x => {
+  | ? adoptive' := ? Children Hole adoptive' eq_refl };
+inject_only_path (Children natural adoptive eq_refl) x with inject_only_triple natural x => {
+  | ? natural' := ? Children natural' adoptive eq_refl }.
+Next Obligation. Qed.
+
+Equations push_left_triple {A lvl len K C}
+  (x : stored_triple A lvl)
+  (t : left_triple A lvl len false K C) :
+  { t' : left_triple A lvl len false K C | push_seq_equality x t t' } :=
+push_left_triple x (Small p s SLeft) with buffer.push x p => {
+  | ? p' := ? Small p' s SLeft };
+push_left_triple x (Green p cd s BLeft) with buffer.push x p => {
+  | ? p' := ? Green p' cd s BLeft };
+push_left_triple x (Yellow p pkt s BLeft) with buffer.push x p => {
+  | ? p' := ? Yellow p' pkt s BLeft };
+push_left_triple x (Orange p pkt s BLeft) with buffer.push x p => {
+  | ? p' := ? Orange p' pkt s BLeft };
+push_left_triple x (Red p cd s BLeft) with buffer.push x p => {
+  | ? p' := ? Red p' cd s BLeft }.
+
+Equations inject_right_triple {A lvl len K C} 
+  (t : right_triple A lvl len false K C) 
+  (x : stored_triple A lvl) :
+  { t' : right_triple A lvl len false K C | inject_seq_equality t x t' } :=
+inject_right_triple (Small p s SRight) x with buffer.inject s x => {
+  | ? s' := ? Small p s' SRight };
+inject_right_triple (Green p cd s BRight) x with buffer.inject s x => {
+  | ? s' := ? Green p cd s' BRight };
+inject_right_triple (Yellow p pkt s BRight) x with buffer.inject s x => {
+  | ? s' := ? Yellow p pkt s' BRight };
+inject_right_triple (Orange p pkt s BRight) x with buffer.inject s x => {
+  | ? s' := ? Orange p pkt s' BRight };
+inject_right_triple (Red p cd s BRight) x with buffer.inject s x => {
+  | ? s' := ? Red p cd s' BRight }.
+
+Equations push_left_path {A lvl C} 
+  (x : stored_triple A lvl)
+  (p : path A lvl Left C) :
+  { p' : path A lvl Left C | path_seq p' = stored_triple_seq x ++ path_seq p } :=
+push_left_path x (Children Hole natural eq_refl) with push_left_triple x natural => {
+  | ? natural' := ? Children Hole natural' eq_refl };
+push_left_path x (Children natural adoptive eq_refl) with push_left_triple x natural => {
+  | ? natural' := ? Children natural' adoptive eq_refl }.
+
+Equations inject_right_path {A lvl C}
+  (p : path A lvl Right C)
+  (x : stored_triple A lvl) :
+  { p' : path A lvl Right C | path_seq p' = path_seq p ++ stored_triple_seq x } :=
+inject_right_path (Children Hole natural eq_refl) x with inject_right_triple natural x => {
+  | ? natural' := ? Children Hole natural' eq_refl };
+inject_right_path (Children natural adoptive eq_refl) x with inject_right_triple natural x => {
+  | ? natural' := ? Children natural' adoptive eq_refl }.
+Next Obligation. Qed.
+
+Equations push_ne_cdeque {A lvl C} 
+  (x : stored_triple A lvl) 
+  (cd : non_empty_cdeque A lvl C) :
+  { cd' : non_empty_cdeque A lvl C | ne_cdeque_seq cd' = stored_triple_seq x ++ ne_cdeque_seq cd } :=
+push_ne_cdeque x (Only_path p) with push_only_path x p => {
+  | ? p' := ? Only_path p' };
+push_ne_cdeque x (Pair_green pl pr) with push_left_path x pl => {
+  | ? pl' := ? Pair_green pl' pr };
+push_ne_cdeque x (Pair_red pl pr) with push_left_path x pl => {
+  | ? pl' := ? Pair_red pl' pr }.
+
+Equations inject_ne_cdeque {A lvl C}
+  (cd : non_empty_cdeque A lvl C)
+  (x : stored_triple A lvl) :
+  { cd' : non_empty_cdeque A lvl C | ne_cdeque_seq cd' = ne_cdeque_seq cd ++ stored_triple_seq x } :=
+inject_ne_cdeque (Only_path p) x with inject_only_path p x => {
+  | ? p' := ? Only_path p' };
+inject_ne_cdeque (Pair_green pl pr) x with inject_right_path pr x => {
+  | ? pr' := ? Pair_green pl pr' };
+inject_ne_cdeque (Pair_red pl pr) x with inject_right_path pr x => {
+  | ? pr' := ? Pair_red pl pr' }.
+
+Equations single_triple {A lvl} (x : stored_triple A lvl) :
+  {t : triple A lvl 0 false Only Only green | triple_seq t = stored_triple_seq x } :=
+single_triple x with buffer.single x, buffer.empty => { | ? p, ? s := ? Small p s SOnly }.
+
+Equations only_single {A lvl} (x : stored_triple A lvl) :
+  {cd : non_empty_cdeque A lvl green | ne_cdeque_seq cd = stored_triple_seq x } :=
+only_single x with single_triple x => { | ? t := ? Only_path (Children Hole t eq_refl) }.
+
+Equations single {A lvl} (x : stored_triple A lvl) :
+  {cd : cdeque A lvl green | cdeque_seq cd = stored_triple_seq x } :=
+single x with only_single x => { | ? cd := ? NonEmpty cd }. 
+
+Equations push_cdeque {A lvl C} 
+  (x : stored_triple A lvl) 
+  (cd : cdeque A lvl C) :
+  { cd' : cdeque A lvl C | cdeque_seq cd' = stored_triple_seq x ++ cdeque_seq cd } :=
+push_cdeque x Empty with single x => { | ? cd := ? cd };
+push_cdeque x (NonEmpty cd) with push_ne_cdeque x cd => { | ? cd' := ? NonEmpty cd' }.
+
+Equations inject_cdeque {A lvl C}
+  (cd : cdeque A lvl C)
+  (x : stored_triple A lvl) :
+  { cd' : cdeque A lvl C | cdeque_seq cd' = cdeque_seq cd ++ stored_triple_seq x } :=
+inject_cdeque Empty x with single x => { | ? cd := ? cd };
+inject_cdeque (NonEmpty cd) x with inject_ne_cdeque cd x => { | ? cd' := ? NonEmpty cd' }.
+
+Equations push {A} (x : A) (d : deque A) : 
+  { d' : deque A | deque_seq d' = [x] ++ deque_seq d } :=
+push x (T cd) with push_cdeque (ST_ground x) cd => { | ? cd' := ? T cd' }.
+
+Equations inject {A} (d : deque A) (x : A) :
+  { d' : deque A | deque_seq d' = deque_seq d ++ [x] } :=
+inject (T cd) x with inject_cdeque cd (ST_ground x) => { | ? cd' := ? T cd' }.
+
+Equations push_semi {A lvl} 
+  (x : stored_triple A lvl)
+  (sd : sdeque A lvl) :
+  { sd' : sdeque A lvl | sdeque_seq sd' = stored_triple_seq x ++ sdeque_seq sd } :=
+push_semi x (Sd cd) with push_cdeque x cd => { | ? cd' := ? Sd cd' }.
+
+Equations inject_semi {A lvl}
+  (sd : sdeque A lvl)
+  (x : stored_triple A lvl) :
+  { sd' : sdeque A lvl | sdeque_seq sd' = sdeque_seq sd ++ stored_triple_seq x } :=
+inject_semi (Sd cd) x with inject_cdeque cd x => { | ? cd' := ? Sd cd' }.
+
+Equations push_vector {A lvl n C} 
+  (v : vector (stored_triple A lvl) n)
+  (cd : cdeque A lvl C) :
+  { cd' : cdeque A lvl C |
+    cdeque_seq cd' = concat (map stored_triple_seq (vector_seq v)) ++ cdeque_seq cd } :=
+push_vector V0 cd1 := ? cd1;
+push_vector (V1 a1) cd with push_cdeque a1 cd => { | ? cd1 := ? cd1 };
+push_vector (V2 a1 a2) cd with push_cdeque a2 cd => {
+  | ? cd2 with push_cdeque a1 cd2 => { | ? cd1 := ? cd1 } };
+push_vector (V3 a1 a2 a3) cd with push_cdeque a3 cd => { 
+  | ? cd3 with push_cdeque a2 cd3 => { | ? cd2 with push_cdeque a1 cd2 => { 
+    | ? cd1 := ? cd1 } } };
+push_vector (V4 a1 a2 a3 a4) cd with push_cdeque a4 cd => {
+  | ? cd4 with push_cdeque a3 cd4 => { | ? cd3 with push_cdeque a2 cd3 => {
+    | ? cd2 with push_cdeque a1 cd2 => { | ? cd1 := ? cd1 } } } };
+push_vector (V5 a1 a2 a3 a4 a5) cd with push_cdeque a5 cd => {
+  | ? cd5 with push_cdeque a4 cd5 => { | ? cd4 with push_cdeque a3 cd4 => {
+    | ? cd3 with push_cdeque a2 cd3 => { | ? cd2 with push_cdeque a1 cd2 => {
+      | ? cd1 := ? cd1 } } } } };
+push_vector (V6 a1 a2 a3 a4 a5 a6) cd with push_cdeque a6 cd => {
+  | ? cd6 with push_cdeque a5 cd6 => { | ? cd5 with push_cdeque a4 cd5 => {
+    | ? cd4 with push_cdeque a3 cd4 => { | ? cd3 with push_cdeque a2 cd3 => {
+      | ? cd2 with push_cdeque a1 cd2 => { | ? cd1 := ? cd1 } } } } } }.
+
+Equations inject_vector {A lvl n C} 
+  (cd : cdeque A lvl C)
+  (v : vector (stored_triple A lvl) n) :
+  { cd' : cdeque A lvl C |
+    cdeque_seq cd' = cdeque_seq cd ++ concat (map stored_triple_seq (vector_seq v)) } :=
+inject_vector cd0 V0 := ? cd0;
+inject_vector cd (V1 a1) with inject_cdeque cd a1 => { | ? cd1 := ? cd1 };
+inject_vector cd (V2 a1 a2) with inject_cdeque cd a1 => {
+  | ? cd1 with inject_cdeque cd1 a2 => { | ? cd2 := ? cd2 } };
+inject_vector cd (V3 a1 a2 a3) with inject_cdeque cd a1 => { 
+  | ? cd1 with inject_cdeque cd1 a2 => { | ? cd2 with inject_cdeque cd2 a3 => { 
+    | ? cd3 := ? cd3 } } };
+inject_vector cd (V4 a1 a2 a3 a4) with inject_cdeque cd a1 => {
+  | ? cd1 with inject_cdeque cd1 a2 => { | ? cd2 with inject_cdeque cd2 a3 => {
+    | ? cd3 with inject_cdeque cd3 a4 => { | ? cd4 := ? cd4 } } } };
+inject_vector cd (V5 a1 a2 a3 a4 a5) with inject_cdeque cd a1 => {
+  | ? cd1 with inject_cdeque cd1 a2 => { | ? cd2 with inject_cdeque cd2 a3 => {
+    | ? cd3 with inject_cdeque cd3 a4 => { | ? cd4 with inject_cdeque cd4 a5 => {
+      | ? cd5 := ? cd5 } } } } };
+inject_vector cd (V6 a1 a2 a3 a4 a5 a6) with inject_cdeque cd a1 => {
+  | ? cd1 with inject_cdeque cd1 a2 => { | ? cd2 with inject_cdeque cd2 a3 => {
+    | ? cd3 with inject_cdeque cd3 a4 => { | ? cd4 with inject_cdeque cd4 a5 => {
+      | ? cd5 with inject_cdeque cd5 a6 => { | ? cd6 := ? cd6 } } } } } }.
+
+Equations to_pref_left {A lvl C} (cd : non_empty_cdeque A lvl C) : 
+  { pl : pref_left A lvl | pref_left_seq pl = ne_cdeque_seq cd } :=
+to_pref_left (Only_path (Children natur adopt eq_refl)) := 
+  ? Pref_left (Only_child natur) adopt eq_refl;
+to_pref_left (Pair_green (Children natur adopt eq_refl) pr) := 
+  ? Pref_left (Left_child natur pr) adopt eq_refl;
+to_pref_left (Pair_red (Children natur adopt eq_refl) pr) := 
+  ? Pref_left (Left_child natur pr) adopt eq_refl.
+
+Equations to_pref_right {A lvl len nlvl K} 
+  (pkt : packet A lvl len preferred_left K)
+  (t : triple A nlvl 0 false K K green) :
+  nlvl = len + lvl -> 
+  { pr : pref_right A lvl | 
+    pref_right_seq pr = packet_front_seq pkt ++ triple_seq t ++ packet_rear_seq pkt } :=
+to_pref_right (Only_child t1) t2 eq_refl:= ? Pref_right (Only_child t1) t2 eq_refl;
+to_pref_right (Left_child t1 (Children natur adopt eq_refl)) t2 eq_refl := 
+  ? Pref_right (Right_child (Children t1 t2 eq_refl) natur) adopt eq_refl.
+
+Equations no_pref {A lvl len nlvl K}
+  (pkt : packet A lvl len preferred_right K)
+  (t : triple A nlvl 0 false K K green) :
+  nlvl = len + lvl ->
+  { cd : non_empty_cdeque A lvl green | 
+    ne_cdeque_seq cd = packet_front_seq pkt ++ triple_seq t ++ packet_rear_seq pkt } :=
+no_pref (Only_child t1) t2 eq_refl := ? Only_path (Children t1 t2 eq_refl);
+no_pref (Right_child pl t1) t2 eq_refl := ? Pair_green pl (Children t1 t2 eq_refl).
+
+Equations make_child {A lvl len nlvl pref K G R}
+  (pkt : packet A lvl len pref K)
+  (t : triple A nlvl 0 false K K (Mix G NoYellow NoOrange R)) :
+  nlvl = len + lvl ->
+  { sd : sdeque A lvl | 
+    sdeque_seq sd = packet_front_seq pkt ++ triple_seq t ++ packet_rear_seq pkt } :=
+make_child (Only_child t1) t2 eq_refl :=
+  ? Sd (NonEmpty (Only_path (Children t1 t2 eq_refl)));
+make_child (Left_child t1 pr) t2 eq_refl :=
+  ? Sd (NonEmpty (Pair_red (Children t1 t2 eq_refl) pr));
+make_child (G := SomeGreen) (R := NoRed) (Right_child pl t1) t2 eq_refl :=
+  ? Sd (NonEmpty (Pair_green pl (Children t1 t2 eq_refl)));
+make_child (G := NoGreen) (R := SomeRed) (Right_child pl t1) t2 eq_refl :=
+  ? Sd (NonEmpty (Pair_red pl (Children t1 t2 eq_refl))).
+
+#[local] Obligation Tactic :=
+  try first [ done | 
+    cbn beta iota delta zeta; intros; 
+    autorewrite with rlist;
+    try simp buffer_seq in *;
+    hauto db:rlist ].
+ 
+Equations push_child {A lvl len nlvl pref K G R} 
+  (x : stored_triple A lvl) 
+  (pkt : packet A lvl len pref K) 
+  (t : triple A nlvl 0 false K K (Mix G NoYellow NoOrange R)) :
+  nlvl = len + lvl ->
+  { '(pkt', t') : packet A lvl len pref K * 
+                  triple A nlvl 0 false K K (Mix G NoYellow NoOrange R) | 
+    packet_front_seq pkt' ++ triple_seq t' ++ packet_rear_seq pkt' =
+      stored_triple_seq x ++ 
+      packet_front_seq pkt ++ triple_seq t ++ packet_rear_seq pkt } :=
+push_child x (Only_child Hole) t eq_refl with push_only_triple x t => {
+  | ? t' := ? (Only_child Hole, t') };
+push_child x (Only_child t1) t2 eq_refl with push_only_triple x t1 => {
+  | ? t1' := ? (Only_child t1', t2) };
+push_child x (Left_child Hole pr) t eq_refl with push_left_triple x t => {
+  | ? t' := ? (Left_child Hole pr, t') };
+push_child x (Left_child t1 pr) t2 eq_refl with push_left_triple x t1 => {
+  | ? t1' := ? (Left_child t1' pr, t2) };
+push_child x (Right_child pl t1) t2 eq_refl with push_left_path x pl => {
+  | ? pl' := ? (Right_child pl' t1, t2) }.
+
+Equations inject_child {A lvl len nlvl pref K G R} 
+  (pkt : packet A lvl len pref K)
+  (t : triple A nlvl 0 false K K (Mix G NoYellow NoOrange R)) 
+  (x : stored_triple A lvl) :
+  nlvl = len + lvl ->
+  { '(pkt', t') : packet A lvl len pref K * 
+                  triple A nlvl 0 false K K (Mix G NoYellow NoOrange R) | 
+    packet_front_seq pkt' ++ triple_seq t' ++ packet_rear_seq pkt' =
+      packet_front_seq pkt ++ triple_seq t ++ packet_rear_seq pkt ++
+      stored_triple_seq x } :=
+inject_child (Only_child Hole) t x eq_refl with inject_only_triple t x => {
+  | ? t' := ? (Only_child Hole, t') };
+inject_child (Only_child t1) t2 x eq_refl with inject_only_triple t1 x => {
+  | ? t1' := ? (Only_child t1', t2) };
+inject_child (Left_child t1 pr) t2 x eq_refl with inject_right_path pr x => {
+  | ? pr' := ? (Left_child t1 pr', t2) };
+inject_child (Right_child pl Hole) t x eq_refl with inject_right_triple t x => {
+  | ? t' := ? (Right_child pl Hole, t') };
+inject_child (Right_child pl t1) t2 x eq_refl with inject_right_triple t1 x => {
+  | ? t1' := ? (Right_child pl t1', t2) }.
+
+Equations stored_left {A lvl q C} 
+  (p : prefix A lvl (5 + q))
+  (cd : cdeque A (S lvl) C) 
+  (s : suffix A lvl 2)
+  (b : buffer_12 A lvl) :
+  { '(p', x) : prefix A lvl 2 * stored_triple A (S lvl) | 
+    buffer_seq p' ++ stored_triple_seq x = 
+      buffer_seq p ++ cdeque_seq cd ++ buffer_seq s ++ buffer_12_seq b } :=
+stored_left p cd s (x, v) with buffer.inject s x => {
+  | ? s1 with buffer.inject_vector s1 v => {
+    | ? s2 with buffer.pop2 p => {
+      | ? (x1, x2, p1) with buffer.pair x1 x2 => {
+        | ? p2 := ? (p2, ST_triple p1 cd s2) } } } }.
+
+Equations stored_right {A lvl q C} 
+  (b : buffer_12 A lvl)
+  (p : prefix A lvl 2)
+  (cd : cdeque A (S lvl) C)
+  (s : suffix A lvl (5 + q)) :
+  { '(x, s') : stored_triple A (S lvl) * suffix A lvl 2 | 
+    stored_triple_seq x ++ buffer_seq s' =
+      buffer_12_seq b ++ buffer_seq p ++ cdeque_seq cd ++ buffer_seq s } :=
+stored_right (x, v) p cd s with buffer.push_vector v p => {
+  | ? p1 with buffer.push x p1 => {
+    | ? p2 with buffer.eject2 s => {
+      | ? (s1, x1, x2) with buffer.pair x1 x2 => {
+        | ? s2 := ? (ST_triple p2 cd s1, s2) } } } }.
+
+#[local] Obligation Tactic :=
+  try first [ done | 
+    cbn beta iota delta zeta; intros; 
+    try simp triple_seq in *;
+    autorewrite with rlist;
+    try simp buffer_seq in *;
+    hauto db:rlist ].
+
+Equations extract_stored_left {A lvl C} 
+  (p : path A lvl Left C) (b : buffer_12 A lvl) :
+  { '(s, x) : suffix A lvl 2 * stored_triple A (S lvl) | 
+    buffer_seq s ++ stored_triple_seq x = path_seq p ++ buffer_12_seq b } :=
+extract_stored_left (Children Hole (Small p s SLeft) eq_refl) b
+  with stored_left p Empty s b => { | ? (s', x) := ? (s', x) };
+extract_stored_left (Children Hole (Green p cd s BLeft) eq_refl) b 
+  with stored_left p (NonEmpty cd) s b => { | ? (s', x) := ? (s', x) };
+extract_stored_left (Children (Yellow p pkt s BLeft) t eq_refl) b
+  with make_child pkt t _ => {
+    | ? Sd cd with stored_left p cd s b => { | ? (s', x) := ? (s', x) } };
+extract_stored_left (Children (Orange p pkt s BLeft) t eq_refl) b
+  with make_child pkt t _ => {
+    | ? Sd cd with stored_left p cd s b => { | ? (s', x) := ? (s', x) } };
+extract_stored_left (Children Hole (Red p cd s BLeft) eq_refl) b
+  with stored_left p (NonEmpty cd) s b => { | ? (s', x) := ? (s', x) }.
+
+Equations extract_stored_right {A lvl C}
+  (b : buffer_12 A lvl) (p : path A lvl Right C) :
+  { '(x, s) : stored_triple A (S lvl) * suffix A lvl 2 | 
+    stored_triple_seq x ++ buffer_seq s = buffer_12_seq b ++ path_seq p } :=
+extract_stored_right b (Children Hole (Small p s SRight) eq_refl)
+  with stored_right b p Empty s => { | ? (x, s') := ? (x, s') };
+extract_stored_right b (Children Hole (Green p cd s BRight) eq_refl) 
+  with stored_right b p (NonEmpty cd) s => { | ? (x, s') := ? (x, s') };
+extract_stored_right b (Children (Yellow p pkt s BRight) t eq_refl)
+  with make_child pkt t _ => {
+    | ? Sd cd with stored_right b p cd s => { | ? (x, s') := ? (x, s') } };
+extract_stored_right b (Children (Orange p pkt s BRight) t eq_refl)
+  with make_child pkt t _ => {
+    | ? Sd cd with stored_right b p cd s => { | ? (x, s') := ? (x, s') } };
+extract_stored_right b (Children Hole (Red p cd s BRight) eq_refl)
+  with stored_right b p (NonEmpty cd) s => { | ? (x, s') := ? (x, s') }.
+
+Equations left_of_pair {A lvl C1 C2}
+  (pl : path A lvl Left C1) (pr : path A lvl Right C2) :
+  { p : path A lvl Left C1 | path_seq p = path_seq pl ++ path_seq pr } :=
+left_of_pair (Children Hole (Small p s SLeft) eq_refl) pr 
+  with buffer.two s => { | ? (x1, x2) with buffer.inject p x1 => {
+    | ? p' with extract_stored_right (x2, V0) pr => {
+      | ? (stored, s') with single_triple stored => {
+        | ? t := ? Children (Orange p' (Only_child Hole) s' BLeft) t eq_refl } } } };
+left_of_pair (Children Hole (Green p cd s BLeft) eq_refl) pr
+  with buffer.two s => { | ? (x1, x2) with extract_stored_right (x1, V1 x2) pr => {
+    | ? (stored, s') with inject_ne_cdeque cd stored => {
+      | ? cd' := ? Children Hole (Green p cd' s' BLeft) eq_refl } } };
+left_of_pair (Children (Yellow p pkt s BLeft) t eq_refl) pr 
+  with buffer.two s => { | ? (x1, x2) with extract_stored_right (x1, V1 x2) pr => {
+    | ? (stored, s') with inject_child pkt t stored _ => {
+      | ? (pkt', t') := ? Children (Yellow p pkt' s' BLeft) t' eq_refl } } };
+left_of_pair (Children (Orange p pkt s BLeft) t eq_refl) pr
+  with buffer.two s => { | ? (x1, x2) with extract_stored_right (x1, V1 x2) pr => {
+    | ? (stored, s') with inject_child pkt t stored _ => {
+      | ? (pkt', t') := ? Children (Orange p pkt' s' BLeft) t' eq_refl } } };
+left_of_pair (Children Hole (Red p cd s BLeft) eq_refl) pr 
+  with buffer.two s => { | ? (x1, x2) with extract_stored_right (x1, V1 x2) pr => {
+    | ? (stored, s') with inject_ne_cdeque cd stored => {
+      | ? cd' := ? Children Hole (Red p cd' s' BLeft) eq_refl } } }.
+Next Obligation. Qed.
 Next Obligation.
-  cbn; intros * Hpnat *; simp triple_seq in *; autorewrite with rlist in *. 
+  cbn; intros; autorewrite with rlist.
+  simp buffer_seq in *; aac_rewrite y1.
+  hauto db:rlist.
+Qed.
+Next Obligation.
+  cbn; intros; autorewrite with rlist.
+  simp buffer_seq in *; aac_rewrite y1.
+  hauto db:rlist.
+Qed.
 
+Equations right_of_pair {A lvl C1 C2} 
+  (pl : path A lvl Left C1) (pr : path A lvl Right C2) :
+  { p : path A lvl Right C2 | path_seq p = path_seq pl ++ path_seq pr } :=
+right_of_pair pl (Children Hole (Small p s SRight) eq_refl) 
+  with buffer.two p => { | ? (x1, x2) with buffer.push x2 s => {
+    | ? s' with extract_stored_left pl (x1, V0) => {
+      | ? (p', stored) with single_triple stored => {
+        | ? t := ? Children (Orange p' (Only_child Hole) s' BRight) t eq_refl } } } };
+right_of_pair pl (Children Hole (Green p cd s BRight) eq_refl)
+  with buffer.two p => { | ? (x1, x2) with extract_stored_left pl (x1, V1 x2) => {
+    | ? (p', stored) with push_ne_cdeque stored cd => {
+      | ? cd' := ? Children Hole (Green p' cd' s BRight) eq_refl } } };
+right_of_pair pl (Children (Yellow p pkt s BRight) t eq_refl)
+  with buffer.two p => { | ? (x1, x2) with extract_stored_left pl (x1, V1 x2) => {
+    | ? (p', stored) with push_child stored pkt t _ => {
+      | ? (pkt', t') := ? Children (Yellow p' pkt' s BRight) t' eq_refl } } };
+right_of_pair pl (Children (Orange p pkt s BRight) t eq_refl)
+  with buffer.two p => { | ? (x1, x2) with extract_stored_left pl (x1, V1 x2) => {
+    | ? (p', stored) with push_child stored pkt t _ => {
+      | ? (pkt', t') := ? Children (Orange p' pkt' s BRight) t' eq_refl } } };
+right_of_pair pl (Children Hole (Red p cd s BRight) eq_refl)
+  with buffer.two p => { | ? (x1, x2) with extract_stored_left pl (x1, V1 x2) => {
+    | ? (p', stored) with push_ne_cdeque stored cd => {
+      | ? cd' := ? Children Hole (Red p' cd' s BRight) eq_refl } } }.
+Next Obligation.
+  cbn; intros; simp triple_seq in *; autorewrite with rlist.
+  simp packet_front_seq packet_rear_seq in *; autorewrite with rlist.
+  aac_rewrite e0; aac_rewrite y0; simp buffer_seq.
+  hauto db:rlist.
+Qed.
+Next Obligation.
+  cbn; intros; simp triple_seq in *; autorewrite with rlist.
+  simp buffer_seq in *; aac_rewrite e; aac_rewrite y0.
+  hauto db:rlist.
+Qed.
+Next Obligation.
+  cbn; intros; simp triple_seq in *; autorewrite with rlist.
+  simp buffer_seq in *; aac_rewrite e; aac_rewrite y0.
+  hauto db:rlist.
+Qed.
+Next Obligation.
+  cbn; intros; simp triple_seq in *; autorewrite with rlist.
+  aac_rewrite y1; aac_rewrite y0; simp buffer_seq.
+  hauto db:rlist.
+Qed.
+Next Obligation.
+  cbn; intros; simp triple_seq in *; autorewrite with rlist.
+  aac_rewrite y1; aac_rewrite y0; simp buffer_seq.
+  hauto db:rlist.
+Qed.
 
-let push_only_path
-: type a c. a -> (a, c, only) path -> (a, c, only) path
-= fun x (Path (only, kont)) ->
-  match is_hole only, only with
-  | Is_hole, HOLE -> Path (only, push_only_triple x kont)
-  | Not_hole, _   -> Path (push_only_triple x only, kont)
+Equations left_of_only {A lvl C} (p : path A lvl Only C) :
+  { p' : path_attempt A lvl Left C | path_attempt_seq p' = path_seq p } :=
+left_of_only (Children Hole (Small p _ SOnly) eq_refl) 
+  with buffer.has5p2 p => {
+    | ? inl v := ? ZeroSix v;
+    | ? inr (p', x1, x2) with buffer.pair x1 x2 => {
+      | ? s := ? Ok (Children Hole (Small p' s SLeft) eq_refl) } };
+left_of_only (Children Hole (Green p cd s BOnly) eq_refl) 
+  with buffer.eject2 s => { | ? (s1, x1, x2) with buffer.pair x1 x2 => {
+    | ? s' with inject_ne_cdeque cd (ST_small s1) => {
+      | ? cd' := ? Ok (Children Hole (Green p cd' s' BLeft) eq_refl) } } };
+left_of_only (Children (Yellow p pkt s BOnly) t eq_refl) 
+  with buffer.eject2 s => { | ? (s1, x1, x2) with buffer.pair x1 x2 => {
+    | ? s' with inject_child pkt t (ST_small s1) _ => {
+      | ? (pkt', t') := ? Ok (Children (Yellow p pkt' s' BLeft) t' eq_refl) } } };
+left_of_only (Children (Orange p pkt s BOnly) t eq_refl)
+  with buffer.eject2 s => { | ? (s1, x1, x2) with buffer.pair x1 x2 => {
+    | ? s' with inject_child pkt t (ST_small s1) _ => {
+      | ? (pkt', t') := ? Ok (Children (Orange p pkt' s' BLeft) t' eq_refl) } } };
+left_of_only (Children Hole (Red p cd s BOnly) eq_refl)
+  with buffer.eject2 s => { | ? (s1, x1, x2) with buffer.pair x1 x2 => {
+    | ? s' with inject_ne_cdeque cd (ST_small s1) => {
+      | ? cd' := ? Ok (Children Hole (Red p cd' s' BLeft) eq_refl) } } }.
+Next Obligation.
+  cbn; intros; autorewrite with rlist; simp buffer_seq in *.
+  aac_rewrite y0; hauto db:rlist.
+Qed.
+Next Obligation.
+  cbn; intros; autorewrite with rlist; simp buffer_seq in *.
+  aac_rewrite y0; hauto db:rlist.
+Qed.
+
+Equations right_of_only {A lvl C} (p : path A lvl Only C) :
+  { p' : path_attempt A lvl Right C | path_attempt_seq p' = path_seq p } :=
+right_of_only (Children Hole (Small p _ SOnly) eq_refl) 
+  with buffer.has2p5 p => {
+    | ? inl v := ? ZeroSix v;
+    | ? inr (x1, x2, s') with buffer.pair x1 x2 => {
+      | ? p' := ? Ok (Children Hole (Small p' s' SRight) eq_refl) } };
+right_of_only (Children Hole (Green p cd s BOnly) eq_refl) 
+  with buffer.pop2 p => { | ? (x1, x2, p1) with buffer.pair x1 x2 => {
+    | ? p' with push_ne_cdeque (ST_small p1) cd => {
+      | ? cd' := ? Ok (Children Hole (Green p' cd' s BRight) eq_refl) } } };
+right_of_only (Children (Yellow p pkt s BOnly) t eq_refl)
+  with buffer.pop2 p => { | ? (x1, x2, p1) with buffer.pair x1 x2 => {
+    | ? p' with push_child (ST_small p1) pkt t _ => {
+      | ? (pkt', t') := ? Ok (Children (Yellow p' pkt' s BRight) t' eq_refl) } } };
+right_of_only (Children (Orange p pkt s BOnly) t eq_refl) 
+  with buffer.pop2 p => { | ? (x1, x2, p1) with buffer.pair x1 x2 => {
+    | ? p' with push_child (ST_small p1) pkt t _ => {
+      | ? (pkt', t') := ? Ok (Children (Orange p' pkt' s BRight) t' eq_refl) } } };
+right_of_only (Children Hole (Red p cd s BOnly) eq_refl)
+  with buffer.pop2 p => { | ? (x1, x2, p1) with buffer.pair x1 x2 => {
+    | ? p' with push_ne_cdeque (ST_small p1) cd => {
+      | ? cd' := ? Ok (Children Hole (Red p' cd' s BRight) eq_refl) } } }.
+Next Obligation.
+  cbn; intros; autorewrite with rlist; simp buffer_seq in *.
+  aac_rewrite y0; hauto db:rlist.
+Qed.
+Next Obligation.
+  cbn; intros; autorewrite with rlist; simp buffer_seq in *.
+  aac_rewrite y0; hauto db:rlist.
+Qed.
+
+Equations make_left {A lvl C} (cd : cdeque A lvl C) :
+  { p : path_attempt A lvl Left C | path_attempt_seq p = cdeque_seq cd } :=
+make_left Empty := ? ZeroSix V0;
+make_left (NonEmpty (Only_path p)) with left_of_only p => { | ? p' := ? p' };
+make_left (NonEmpty (Pair_green pl pr)) with left_of_pair pl pr => {
+  | ? p := ? Ok p };
+make_left (NonEmpty (Pair_red pl pr)) with left_of_pair pl pr => {
+  | ? p := ? Any p }.
+
+Equations make_right {A lvl C} (cd : cdeque A lvl C) :
+  { p : path_attempt A lvl Right C | path_attempt_seq p = cdeque_seq cd } :=
+make_right Empty := ? ZeroSix V0;
+make_right (NonEmpty (Only_path p)) with right_of_only p => { | ? p' := ? p' };
+make_right (NonEmpty (Pair_green pl pr)) with right_of_pair pl pr => {
+  | ? p := ? Ok p };
+make_right (NonEmpty (Pair_red pl pr)) with right_of_pair pl pr => {
+  | ? p := ? Any p }.
+
+Equations concat_semi {A lvl} (sd1 sd2 : sdeque A lvl) :
+  { sd : sdeque A lvl | sdeque_seq sd = sdeque_seq sd1 ++ sdeque_seq sd2 } :=
+concat_semi (Sd cd1) (Sd cd2) with make_left cd1 => {
+  | ? ZeroSix v with push_vector v cd2 => {
+    | ? cd := ? Sd cd };
+  | ? Ok pl with make_right cd2 => {
+    | ? ZeroSix v with inject_vector cd1 v => {
+      | ? cd := ? Sd cd };
+    | ? Ok pr := ? Sd (NonEmpty (Pair_red pl pr));
+    | ? Any pr := ? Sd (NonEmpty (Pair_red pl pr)) };
+  | ? Any pl with make_right cd2 => {
+    | ? ZeroSix v with inject_vector cd1 v => {
+      | ? cd := ? Sd cd };
+    | ? Ok pr := ? Sd (NonEmpty (Pair_red pl pr));
+    | ? Any pr := ? Sd (NonEmpty (Pair_red pl pr)) } }.
+
+Equations concat {A} (d1 d2 : deque A) : 
+  { d : deque A | deque_seq d = deque_seq d1 ++ deque_seq d2 } :=
+concat (T cd1) (T cd2) with make_left cd1 => {
+  | ? ZeroSix v with push_vector v cd2 => {
+    | ? cd := ? T cd };
+  | ? Ok pl with make_right cd2 => {
+    | ? ZeroSix v with inject_vector cd1 v => {
+      | ? cd := ? T cd };
+    | ? Ok pr := ? T (NonEmpty (Pair_green pl pr)) } }.
+
+Equations semi_of_left {A lvl C} 
+  (p : path A lvl Left C) 
+  (x1 x2 x3 x4 x5 x6 : stored_triple A lvl) :
+  { sd : sdeque A lvl | 
+    sdeque_seq sd = path_seq p ++ stored_triple_seq x1 ++ stored_triple_seq x2 ++ 
+                                  stored_triple_seq x3 ++ stored_triple_seq x4 ++ 
+                                  stored_triple_seq x5 ++ stored_triple_seq x6 } :=
+semi_of_left (Children Hole (Small p s SLeft) eq_refl) x1 x2 x3 x4 x5 x6 
+  with buffer.two s => { | ? (y1, y2) with buffer.inject2 p y1 y2 => {
+    | ? p1 with buffer.inject6 p1 x1 x2 x3 x4 x5 x6, buffer.empty => {
+      | ? p2, ? s2 := 
+      ? Sd (NonEmpty (Only_path (Children Hole (Small p2 s2 SOnly) eq_refl))) } } };
+semi_of_left (Children Hole (Green p cd s BLeft) eq_refl) x1 x2 x3 x4 x5 x6 
+  with buffer.inject6 s x1 x2 x3 x4 x5 x6 => {
+    | ? s' := 
+    ? Sd (NonEmpty (Only_path (Children Hole (Green p cd s' BOnly) eq_refl))) };
+semi_of_left (Children (Yellow p pkt s BLeft) t eq_refl) x1 x2 x3 x4 x5 x6 
+  with buffer.inject6 s x1 x2 x3 x4 x5 x6 => {
+    | ? s' := 
+    ? Sd (NonEmpty (Only_path (Children (Yellow p pkt s' BOnly) t eq_refl))) };
+semi_of_left (Children (Orange p pkt s BLeft) t eq_refl) x1 x2 x3 x4 x5 x6
+  with buffer.inject6 s x1 x2 x3 x4 x5 x6 => {
+    | ? s' :=
+    ? Sd (NonEmpty (Only_path (Children (Orange p pkt s' BOnly) t eq_refl))) };
+semi_of_left (Children Hole (Red p cd s BLeft) eq_refl) x1 x2 x3 x4 x5 x6
+  with buffer.inject6 s x1 x2 x3 x4 x5 x6 => {
+    | ? s' := 
+    ? Sd (NonEmpty (Only_path (Children Hole (Red p cd s' BOnly) eq_refl))) }.
+Next Obligation.
+  cbn; intros; simp triple_seq in *; autorewrite with rlist; simp buffer_seq in *. 
+  rewrite <-y; autorewrite with rlist; hauto db:rlist.
+Qed.
+
+Equations semi_of_right {A lvl C} 
+  (x1 x2 x3 x4 x5 x6 : stored_triple A lvl) 
+  (p : path A lvl Right C) :
+  { sd : sdeque A lvl | 
+    sdeque_seq sd = stored_triple_seq x1 ++ stored_triple_seq x2 ++
+                    stored_triple_seq x3 ++ stored_triple_seq x4 ++
+                    stored_triple_seq x5 ++ stored_triple_seq x6 ++ path_seq p } :=
+semi_of_right x1 x2 x3 x4 x5 x6 (Children Hole (Small p s SRight) eq_refl) 
+  with buffer.two p => { | ? (y1, y2) with buffer.push2 y1 y2 s => {
+    | ? s1 with buffer.push6 x1 x2 x3 x4 x5 x6 s1, buffer.empty => {
+      | ? p2, ? s2 := 
+      ? Sd (NonEmpty (Only_path (Children Hole (Small p2 s2 SOnly) eq_refl))) } } };
+semi_of_right x1 x2 x3 x4 x5 x6 (Children Hole (Green p cd s BRight) eq_refl)
+  with buffer.push6 x1 x2 x3 x4 x5 x6 p => {
+    | ? p' :=
+    ? Sd (NonEmpty (Only_path (Children Hole (Green p' cd s BOnly) eq_refl))) };
+semi_of_right x1 x2 x3 x4 x5 x6 (Children (Yellow p pkt s BRight) t eq_refl) 
+  with buffer.push6 x1 x2 x3 x4 x5 x6 p => {
+    | ? p' :=
+    ? Sd (NonEmpty (Only_path (Children (Yellow p' pkt s BOnly) t eq_refl))) };
+semi_of_right x1 x2 x3 x4 x5 x6 (Children (Orange p pkt s BRight) t eq_refl)
+  with buffer.push6 x1 x2 x3 x4 x5 x6 p => {
+    | ? p' :=
+    ? Sd (NonEmpty (Only_path (Children (Orange p' pkt s BOnly) t eq_refl))) };
+semi_of_right x1 x2 x3 x4 x5 x6 (Children Hole (Red p cd s BRight) eq_refl)
+  with buffer.push6 x1 x2 x3 x4 x5 x6 p => {
+    | ? p' := 
+    ? Sd (NonEmpty (Only_path (Children Hole (Red p' cd s BOnly) eq_refl))) }.
+
+Equations pop_green_left {A lvl} (p : path A lvl Left green) :
+  { '(x, p') : stored_triple A lvl * path_uncolored A lvl Left | 
+    stored_triple_seq x ++ path_uncolored_seq p' = path_seq p } :=
+pop_green_left (Children Hole (Small p s SLeft) eq_refl) 
+  with buffer.pop p => { | ? (x, p1) with buffer.has5 p1 => {
+    | ? inl (x1, x2, x3, x4) with buffer.two s => { | ? (x5, x6) := 
+      ? (x, Six x1 x2 x3 x4 x5 x6) };
+    | ? inr p2 := ? (x, AnyColor (Children Hole (Small p2 s SLeft) eq_refl)) } };
+pop_green_left (Children Hole (Green p cd s BLeft) eq_refl)
+  with buffer.pop p => { | ? (x, p1) with to_pref_left cd => {
+    | ? Pref_left pkt t eq_refl := 
+      ? (x, AnyColor (Children (Yellow p1 pkt s BLeft) t _)) } };
+pop_green_left (Children (Yellow p pkt s BLeft) t eq_refl) 
+  with buffer.pop p => { | ? (x, p1) with to_pref_right pkt t _ => {
+    | ? Pref_right pkt' t' eq_refl := 
+      ? (x, AnyColor (Children (Orange p1 pkt' s BLeft) t' _)) } };
+pop_green_left (Children (Orange p pkt s BLeft) t eq_refl)
+  with buffer.pop p => { | ? (x, p1) with no_pref pkt t _ => {
+    | ? cd := ? (x, AnyColor (Children Hole (Red p1 cd s BLeft) eq_refl)) } }.
+Next Obligation. Qed.
+Next Obligation. 
+  cbn; intros; autorewrite with rlist; simp buffer_seq in *.
+  aac_rewrite e; hauto db:rlist.
+Qed.
+
+Equations eject_green_right {A lvl} (p : path A lvl Right green) :
+  { '(p', x) : path_uncolored A lvl Right * stored_triple A lvl |
+    path_uncolored_seq p' ++ stored_triple_seq x = path_seq p } :=
+eject_green_right (Children Hole (Small p s SRight) eq_refl)
+  with buffer.eject s => { | ? (s1, x) with buffer.has5 s1 => {
+    | ? inl (x3, x4, x5, x6) with buffer.two p => { | ? (x1, x2) := 
+      ? (Six x1 x2 x3 x4 x5 x6, x) };
+    | ? inr s2 := ? (AnyColor (Children Hole (Small p s2 SRight) eq_refl), x) } };
+eject_green_right (Children Hole (Green p cd s BRight) eq_refl)
+  with buffer.eject s => { | ? (s1, x) with to_pref_left cd => {
+    | ? Pref_left pkt t eq_refl := 
+      ? (AnyColor (Children (Yellow p pkt s1 BRight) t _), x) } };
+eject_green_right (Children (Yellow p pkt s BRight) t eq_refl)
+  with buffer.eject s => { | ? (s1, x) with to_pref_right pkt t _ => {
+    | ? Pref_right pkt' t' eq_refl := 
+      ? (AnyColor (Children (Orange p pkt' s1 BRight) t' _), x) } };
+eject_green_right (Children (Orange p pkt s BRight) t eq_refl)
+  with buffer.eject s => { | ? (s1, x) with no_pref pkt t _ => {
+    | ? cd := ? (AnyColor (Children Hole (Red p cd s1 BRight) eq_refl), x) } }.
+Next Obligation. Qed.
+Next Obligation.
+  cbn; intros; autorewrite with rlist; simp buffer_seq in *.
+  aac_rewrite e; hauto db:rlist.
+Qed.
+
+Equations pop_green {A lvl} (cd : non_empty_cdeque A lvl green) :
+  { '(x, sd) : stored_triple A lvl * sdeque A lvl | 
+    stored_triple_seq x ++ sdeque_seq sd = ne_cdeque_seq cd } :=
+pop_green (Only_path (Children Hole (Small p s SOnly) eq_refl)) 
+  with buffer.pop p => { | ? (x, p1) with buffer.has1 p1 => {
+    | ? None := ? (x, Sd Empty);
+    | ? Some p2 := 
+    ? (x, Sd (NonEmpty (Only_path (Children Hole (Small p2 s SOnly) eq_refl)))) } };
+pop_green (Only_path (Children Hole (Green p cd s BOnly) eq_refl))
+  with buffer.pop p => { | ? (x, p1) with to_pref_left cd => {
+    | ? Pref_left pkt t eq_refl :=
+    ? (x, Sd (NonEmpty (Only_path (Children (Yellow p1 pkt s BOnly) t _)))) } };
+pop_green (Only_path (Children (Yellow p pkt s BOnly) t eq_refl))
+  with buffer.pop p => { | ? (x, p1) with to_pref_right pkt t _ => {
+    | ? Pref_right pkt' t' eq_refl :=
+    ? (x, Sd (NonEmpty (Only_path (Children (Orange p1 pkt' s BOnly) t' _)))) } };
+pop_green (Only_path (Children (Orange p pkt s BOnly) t eq_refl))
+  with buffer.pop p => { | ? (x, p1) with no_pref pkt t _ => 
+    | ? cd := 
+    ? (x, Sd (NonEmpty (Only_path (Children Hole (Red p1 cd s BOnly) eq_refl)))) };
+pop_green (Pair_green pl pr) with pop_green_left pl => {
+  | ? (x, Six x1 x2 x3 x4 x5 x6) with semi_of_right x1 x2 x3 x4 x5 x6 pr => {
+    | ? sd := ? (x, sd) };
+  | ? (x, AnyColor pl') := ? (x, Sd (NonEmpty (Pair_red pl' pr))) }.
+Next Obligation. Qed.
+Next Obligation.
+  cbn; intros; autorewrite with rlist; simp buffer_seq in *.
+  aac_rewrite e; hauto db:rlist.
+Qed.
+
+Equations eject_green {A lvl} (cd : non_empty_cdeque A lvl green) :
+  { '(sd, x) : sdeque A lvl * stored_triple A lvl | 
+    sdeque_seq sd ++ stored_triple_seq x = ne_cdeque_seq cd } :=
+eject_green (Only_path (Children Hole (Small p s SOnly) eq_refl)) 
+  with buffer.eject p => { | ? (p1, x) with buffer.has1 p1 => {
+    | ? None := ? (Sd Empty, x);
+    | ? Some p2 := 
+    ? (Sd (NonEmpty (Only_path (Children Hole (Small p2 s SOnly) eq_refl))), x) } };
+eject_green (Only_path (Children Hole (Green p cd s BOnly) eq_refl))
+  with buffer.eject s => { | ? (s1, x) with to_pref_left cd => {
+    | ? Pref_left pkt t eq_refl :=
+    ? (Sd (NonEmpty (Only_path (Children (Yellow p pkt s1 BOnly) t _))), x) } };
+eject_green (Only_path (Children (Yellow p pkt s BOnly) t eq_refl))
+  with buffer.eject s => { | ? (s1, x) with to_pref_right pkt t _ => {
+    | ? Pref_right pkt' t' eq_refl := 
+    ? (Sd (NonEmpty (Only_path (Children (Orange p pkt' s1 BOnly) t' _))), x) } };
+eject_green (Only_path (Children (Orange p pkt s BOnly) t eq_refl)) 
+  with buffer.eject s => { | ? (s1, x) with no_pref pkt t _ => {
+    | ? cd := 
+    ? (Sd (NonEmpty (Only_path (Children Hole (Red p cd s1 BOnly) eq_refl))), x) } };
+eject_green (Pair_green pl pr) with eject_green_right pr => {
+  | ? (Six x1 x2 x3 x4 x5 x6, x) with semi_of_left pl x1 x2 x3 x4 x5 x6 => {
+    | ? sd := ? (sd, x) };
+  | ? (AnyColor pr', x) := ? (Sd (NonEmpty (Pair_red pl pr')), x) }.
+Next Obligation. Qed.
+Next Obligation. 
+  cbn; intros; autorewrite with rlist; simp buffer_seq in *.
+  aac_rewrite e; hauto db:rlist.
+Qed.
+
+Equations pop_stored {A lvl} (cd : non_empty_cdeque A (S lvl) green) :
+  { uns : unstored A lvl | 
+    unstored_front_seq uns ++ unstored_rear_seq uns = ne_cdeque_seq cd } :=
+pop_stored cd with pop_green cd => {
+  | ? (ST_small p, sd) := ? Unstored p sd
+  | ? (ST_triple p cd1 s, sd) with push_semi (ST_small s) sd => {
+    | ? sd1 with concat_semi (Sd cd1) sd1 => {
+      | ? sd2 := ? Unstored p sd2 } } }.
+
+Equations eject_stored {A lvl} (cd : non_empty_cdeque A (S lvl) green) :
+  { uns : unstored A lvl | 
+    unstored_rear_seq uns ++ unstored_front_seq uns = ne_cdeque_seq cd } :=
+eject_stored cd with eject_green cd => {
+  | ? (sd, ST_small p) := ? Unstored p sd
+  | ? (sd, ST_triple p cd1 s) with inject_semi sd (ST_small p) => {
+    | ? sd1 with concat_semi sd1 (Sd cd1) => {
+      | ? sd2 := ? Unstored s sd2 } } }.
+
+Equations unsandwich_green {A lvl} (cd : non_empty_cdeque A lvl green) :
+  { s : sandwich A lvl | sandwich_seq s = ne_cdeque_seq cd } :=
+unsandwich_green (Only_path (Children Hole (Small p s SOnly) eq_refl)) 
+  with buffer.pop p => { | ? (x1, p1) with buffer.has1 p1 => {
+    | ? None := ? Alone x1;
+    | ? Some p2 with buffer.eject p2 => { | ? (p3, x2) with buffer.has1 p3 => {
+      | ? None := ? Sandwich x1 (Sd Empty) x2;
+      | ? Some p4 := 
+        let only := Only_path (Children Hole (Small p4 s SOnly) eq_refl) in 
+        ? Sandwich x1 (Sd (NonEmpty only)) x2 } } } };
+unsandwich_green (Only_path (Children Hole (Green p cd s BOnly) eq_refl))
+  with buffer.pop p => { | ? (x1, p1) with buffer.eject s => { 
+    | ? (s1, x2) with to_pref_left cd => { | ? Pref_left pkt t eq_refl := 
+    (* If we remove eq_refl, equations fail with "Constructor is applied to too 
+       many arguments", when in fact it is the opposite. *)
+      let only := Only_path (Children (Yellow p1 pkt s1 BOnly) t _) in 
+      ? Sandwich x1 (Sd (NonEmpty only)) x2 } } };
+unsandwich_green (Only_path (Children (Yellow p pkt s BOnly) t eq_refl))
+  with buffer.pop p => { | ? (x1, p1) with buffer.eject s => {
+    | ? (s1, x2) with to_pref_right pkt t _ => { | ? Pref_right pkt' t' eq_refl := 
+      let only := Only_path (Children (Orange p1 pkt' s1 BOnly) t' _) in 
+      ? Sandwich x1 (Sd (NonEmpty only)) x2 } } };
+unsandwich_green (Only_path (Children (Orange p pkt s BOnly) t eq_refl))
+  with buffer.pop p => { | ? (x1, p1) with buffer.eject s => {
+    | ? (s1, x2) with no_pref pkt t _ => { | ? cd := 
+      let only := Only_path (Children Hole (Red p1 cd s1 BOnly) eq_refl) in
+      ? Sandwich x1 (Sd (NonEmpty only)) x2 } } };
+unsandwich_green (Pair_green pl pr) with pop_green_left pl => {
+  | ? (x1, Six x2 x3 x4 x5 x6 x7) with eject_green_right pr => {
+    | ? (Six x8 x9 x10 x11 x12 x13, x14) with buffer.empty => {
+      | ? b with buffer.push6 x8 x9 x10 x11 x12 x13 b => {
+        | ? b1 with buffer.push6 x2 x3 x4 x5 x6 x7 b1 => {
+          | ? b2 := 
+            let only := Only_path (Children Hole (Small b2 b SOnly) eq_refl) in
+            ? Sandwich x1 (Sd (NonEmpty only)) x14 } } };
+    | ? (AnyColor pr1, x8) with semi_of_right x2 x3 x4 x5 x6 x7 pr1 => {
+      | ? sd := ? Sandwich x1 sd x8 } };
+  | ? (x1, AnyColor pl1) with eject_green_right pr => {
+    | ? (Six x2 x3 x4 x5 x6 x7, x8) with semi_of_left pl1 x2 x3 x4 x5 x6 x7 => {
+      | ? sd := ? Sandwich x1 sd x8 };
+    | ? (AnyColor pr1, x2) := 
+      ? Sandwich x1 (Sd (NonEmpty (Pair_red pl1 pr1))) x2 } }.
+Next Obligation.
+  cbn; intros; simp triple_seq in *; autorewrite with rlist; simp buffer_seq in *.
+  pose (buffer.empty_buffer s) as H; rewrite H; cbn.
+  rewrite <-y; rewrite <-e; hauto db:rlist.
+Qed.
+Next Obligation.
+  cbn; intros; simp triple_seq in *; autorewrite with rlist; simp buffer_seq in *.
+  pose (buffer.empty_buffer s) as H; rewrite H; cbn.
+  rewrite <-y; rewrite <-e; hauto db:rlist.
+Qed.
+Next Obligation. Qed.
+Next Obligation.
+  cbn; intros; autorewrite with rlist; simp buffer_seq in *.
+  aac_rewrite e; hauto db:rlist.
+Qed.
+
+Equations unsandwich_stored {A lvl} (cd : non_empty_cdeque A (S lvl) green) :
+  { us : unstored_sandwich A lvl | unstored_sandwich_seq us = ne_cdeque_seq cd } :=
+unsandwich_stored cd with unsandwich_green cd => {
+  | ? Alone (ST_small p) := ? Unstored_alone p;
+  | ? Alone (ST_triple p cd1 s) := ? Unstored_sandwich p (Sd cd1) s;
+  | ? Sandwich (ST_small p) sd (ST_small s) := ? Unstored_sandwich p sd s;
+  | ? Sandwich (ST_small p) sd (ST_triple p1 cd1 s) 
+    with inject_semi sd (ST_small p1) => { | ? sd1 with concat_semi sd1 (Sd cd1) => {
+      | ? sd2 := ? Unstored_sandwich p sd2 s } };
+  | ? Sandwich (ST_triple p cd1 s1) sd (ST_small s) 
+    with push_semi (ST_small s1) sd => { | ? sd1 with concat_semi (Sd cd1) sd1 => {
+      | ? sd2 := ? Unstored_sandwich p sd2 s } };
+  | ? Sandwich (ST_triple p cdl sl) sd (ST_triple pr cdr s) 
+    with push_semi (ST_small sl) sd => { 
+      | ? sd1 with inject_semi sd1 (ST_small pr) => {
+        | ? sd2 with concat_semi (Sd cdl) sd2 => { 
+          | ? sd3 with concat_semi sd3 (Sd cdr) => {
+            | ? sd4 := ? Unstored_sandwich p sd4 s } } } } }.
+
+Equations only_small {A lvl qp qs} 
+  (p : prefix A lvl (8 + qp)) 
+  (s : suffix A lvl (8 + qs)) :
+  { t : triple A lvl 0 false Only Only green | 
+    triple_seq t = buffer_seq p ++ buffer_seq s } :=
+only_small p s with buffer.has3p8 s => {
+  | ? inl (x1, x2, x3, x4, x5, x6, x7, x8, v) 
+    with buffer.inject8 p x1 x2 x3 x4 x5 x6 x7 x8 => {
+      | ? p1 with buffer.inject_vector p1 v, buffer.empty => {
+          | ? p2, ? s2 := ? Small p2 s2 SOnly } };
+  | ? inr (x1, x2, x3, s1) with buffer.triple x1 x2 x3 => {
+    | ? b with only_single (ST_small b) => {
+      | ? cd := ? Green p cd s1 BOnly } } }.
+Next Obligation.
+  cbn; intros; simp triple_seq in *; autorewrite with rlist. 
+  autorewrite with rlist in e1; simp buffer_seq in *; hauto db:rlist.
+Qed.
+
+Equations only_green {A lvl qp qs} 
+  (p : prefix A lvl (8 + qp))
+  (sd : sdeque A (S lvl))
+  (s : suffix A lvl (8 + qs)) :
+  { t : triple A lvl 0 false Only Only green | 
+    triple_seq t = buffer_seq p ++ sdeque_seq sd ++ buffer_seq s } :=
+only_green p (Sd Empty) s with only_small p s => { | ? t := ? t };
+only_green p (Sd (NonEmpty cd)) s := ? Green p cd s BOnly.
+
+Local Ltac rewrite_seq :=
+  repeat 
+  match goal with 
+  | H : _ = seq _ |- _ => rewrite <-H
+  end.
+
+#[local] Obligation Tactic := idtac.
+
+(* #[local] Obligation Tactic := 
+  cbn; intros; simp triple_seq in *; 
+  autorewrite with rlist; simp buffer_seq in *;
+  rewrite_seq; hauto db:rlist. *)
+
+Equations green_of_red_only {A lvl} (t : triple A lvl 0 false Only Only red) :
+  { t' : triple A lvl 0 false Only Only green | triple_seq t' = triple_seq t } :=
+green_of_red_only (Red p cd s BOnly) with buffer.has8 p, buffer.has8 s => {
+  | ? inl (x1, x2, x3, x4, x5, vp), ? inl (y1, y2, y3, y4, y5, vs) 
+    with unsandwich_stored cd => {
+      | ? Unstored_alone center with buffer.push5_vector x1 x2 x3 x4 x5 vp center => {
+        | ? center1 with buffer.inject5_vector center1 y1 y2 y3 y4 y5 vs, buffer.empty => {
+            | ? center2, ? empty := ? Small center2 empty SOnly } };
+      | ? Unstored_sandwich p1 sd s1 
+        with buffer.push5_vector x1 x2 x3 x4 x5 vp p1 => {
+          | ? p2 with buffer.inject5_vector s1 y1 y2 y3 y4 y5 vs => {
+            | ? s2 with only_green p2 sd s2 => { | ? t := ? t } } } };
+  | ? inl (x1, x2, x3, x4, x5, vp), ? inr s1 with pop_stored cd => {
+    | ? Unstored p1 sd with buffer.push5_vector x1 x2 x3 x4 x5 vp p1 => {
+      | ? p2 with only_green p2 sd s1 => { | ? t := ? t } } };
+  | ? inr p1, ? inl (y1, y2, y3, y4, y5, vs) with eject_stored cd => {
+    | ? Unstored s1 sd with buffer.inject5_vector s1 y1 y2 y3 y4 y5 vs => {
+      | ? s2 with only_green p1 sd s2 => { | ? t := ? t } } };
+  | ? inr p1, ? inr s1 := ? Green p1 cd s1 BOnly }.
+Next Obligation.
+  cbn; intros; simp triple_seq in *; autorewrite with rlist; simp buffer_seq in *.
+  rewrite_seq; hauto db:rlist.
+Qed.
+Next Obligation.
+  cbn; intros; simp triple_seq in *; autorewrite with rlist; simp buffer_seq in *.
+  rewrite_seq; hauto db:rlist.
+Qed.
+Next Obligation.
+  cbn; intros; simp triple_seq in *; autorewrite with rlist; simp buffer_seq in *.
+  rewrite_seq; hauto db:rlist.
+Qed.
+Next Obligation.
+  cbn; intros; simp triple_seq in *; autorewrite with rlist; simp buffer_seq in *.
+  rewrite_seq; hauto db:rlist.
+Qed.
+Next Obligation.
+  cbn; intros; simp triple_seq in *; autorewrite with rlist; simp buffer_seq in *.
+  rewrite_seq; hauto db:rlist.
+Qed.
+
+Equations green_of_red_left {A lvl} (t : triple A lvl 0 false Left Left red) :
+  { t' : triple A lvl 0 false Left Left green | triple_seq t' = triple_seq t } :=
+green_of_red_left (Red p cd s BLeft) with buffer.has8 p => {
+  | ? inl (x1, x2, x3, x4, x5, vp) with pop_stored cd => {
+    | ? Unstored p1 (Sd cd1) with buffer.push5_vector x1 x2 x3 x4 x5 vp p1 => {
+      | ? p2 with cd1 => {
+        | Empty := ? Small p2 s SLeft; 
+        | NonEmpty cd1' := ? Green p2 cd1' s BLeft } } };
+  | ? inr p1 := ? Green p1 cd s BLeft }.
+Next Obligation.
+  cbn; intros; simp triple_seq in *; autorewrite with rlist; simp buffer_seq in *.
+  rewrite_seq; hauto db:rlist.
+Qed.
+Next Obligation.
+  cbn; intros; simp triple_seq in *; autorewrite with rlist; simp buffer_seq in *.
+  rewrite_seq; hauto db:rlist.
+Qed.
+Next Obligation.
+  cbn; intros; simp triple_seq in *; autorewrite with rlist; simp buffer_seq in *.
+  rewrite_seq; hauto db:rlist.
+Qed.
+
+Equations green_of_red_right {A lvl} (t : triple A lvl 0 false Right Right red) :
+  { t' : triple A lvl 0 false Right Right green | triple_seq t' = triple_seq t } :=
+green_of_red_right (Red p cd s BRight) with buffer.has8 s => {
+  | ? inl (y1, y2, y3, y4, y5, vs) with eject_stored cd => {
+    | ? Unstored s1 (Sd cd1) with buffer.inject5_vector s1 y1 y2 y3 y4 y5 vs => {
+      | ? s2 with cd1 => {
+        | Empty := ? Small p s2 SRight;
+        | NonEmpty cd1' := ? Green p cd1' s2 BRight } } };
+  | ? inr s1 := ? Green p cd s1 BRight }.
+Next Obligation.
+  cbn; intros; simp triple_seq in *; autorewrite with rlist; simp buffer_seq in *.
+  rewrite_seq; hauto db:rlist.
+Qed.
+Next Obligation.
+  cbn; intros; simp triple_seq in *; autorewrite with rlist; simp buffer_seq in *.
+  rewrite_seq; hauto db:rlist.
+Qed.
+Next Obligation.
+  cbn; intros; simp triple_seq in *; autorewrite with rlist; simp buffer_seq in *.
+  rewrite_seq; hauto db:rlist.
+Qed.
+
+#[local] Obligation Tactic :=
+  try first [ done | 
+    cbn beta iota delta zeta; intros; 
+    try simp triple_seq in *;
+    autorewrite with rlist;
+    try simp buffer_seq in *;
+    hauto db:rlist ].
+
+Equations ensure_green {A lvl} (K : kind) (G : green_hue) (R : red_hue) 
+  (t : triple A lvl 0 false K K (Mix G NoYellow NoOrange R)) :
+  { t' : triple A lvl 0 false K K green | triple_seq t' = triple_seq t } :=
+ensure_green _ SomeGreen NoRed t := ? t;
+ensure_green Only NoGreen SomeRed t with green_of_red_only t => { 
+  | ? t' := ? t' };
+ensure_green Left NoGreen SomeRed t with green_of_red_left t => {
+  | ? t' := ? t' };
+ensure_green Right NoGreen SomeRed t with green_of_red_right t => {
+  | ? t' := ? t' }.
+Arguments ensure_green {A lvl K G R}.
+
+Equations ensure_green_path {A lvl K C} (p : path A lvl K C) :
+  { p' : path A lvl K green | path_seq p' = path_seq p } :=
+ensure_green_path (Children natur adopt eq_refl) with ensure_green adopt => {
+  | ? adopt' := ? Children natur adopt' eq_refl }.
+Next Obligation.
+  cbn; intros; rewrite e; reflexivity.
+Qed.
+
+Equations ensure_green_cdeque {A lvl C} (cd : non_empty_cdeque A lvl C) :
+  { cd' : non_empty_cdeque A lvl green | ne_cdeque_seq cd' = ne_cdeque_seq cd } :=
+ensure_green_cdeque (Only_path p) with ensure_green_path p => {
+  | ? p' := ? Only_path p' };
+ensure_green_cdeque (Pair_green pl pr) := ? Pair_green pl pr;
+ensure_green_cdeque (Pair_red pl pr) 
+  with ensure_green_path pl, ensure_green_path pr => {
+    | ? pl', ? pr' := ? Pair_green pl' pr' }.
+
+Equations regular_of_semi {A} (sd : sdeque A 0) : 
+  { d : deque A | deque_seq d = sdeque_seq sd } :=
+regular_of_semi (Sd Empty) := ? T Empty;
+regular_of_semi (Sd (NonEmpty cd)) with ensure_green_cdeque cd => {
+  | ? cd' := ? T (NonEmpty cd') }.
+
+Equations pop {A} (d : deque A) : 
+  { o : option (A * deque A) | 
+    match o with 
+    | None => []
+    | Some (x, d') => [x] ++ deque_seq d' 
+    end = deque_seq d } := 
+pop (T Empty) := ? None;
+pop (T (NonEmpty cd)) with pop_green cd => {
+  | ? (ST_ground x, sd) with regular_of_semi sd => {
+    | ? d' := ? Some (x, d') } }.
+
+Equations eject {A} (d : deque A) :
+  { o : option (deque A * A) | 
+    match o with 
+    | None => [] 
+    | Some (d', x) => deque_seq d' ++ [x] 
+    end = deque_seq d } :=
+eject (T Empty) := ? None;
+eject (T (NonEmpty cd)) with eject_green cd => {
+  | ? (sd, ST_ground x) with regular_of_semi sd => {
+    | ? d' := ? Some (d', x) } }.
